Added invariant and removed 'assume's

src/verification/dafny/astar_navfnplanner.dfy
@@ -27,19 +27,51 @@ predicate ValidPotentialMap(pot: PotentialMap, costMap: CostMap)
     pot[i][j].Real? ==> open(costMap, i, j)
 }
 
+predicate ValidCostMap(costMap: CostMap)
+{
+  forall i, j | 0 <= i < costMap.numRows && 0 <= j < costMap.numCols :: costMap.value(Point(i, j)) > 0.0
+}
+
+predicate AdjacentHorizontal(p1: Pose, p2: Pose)
+{
+  (p1.pos.row == p2.pos.row && p1.pos.col == p2.pos.col + 1)
+  || (p1.pos.row == p2.pos.row && p1.pos.col == p2.pos.col - 1)
+}
+
+predicate AdjacentVertical(p1: Pose, p2: Pose)
+{
+  (p1.pos.col == p2.pos.col && p1.pos.row == p2.pos.row - 1)
+  || (p1.pos.col == p2.pos.col && p1.pos.row == p2.pos.row + 1)
+}
+predicate Adjacent(p1: Pose, p2: Pose, costMap: CostMap)
+{
+  AdjacentHorizontal(p1, p2) || AdjacentVertical(p1, p2)
+}
+
+predicate HasSomeAdjacentReal(p: Pose, pot: PotentialMap, numRows: nat, numCols: nat)
+  requires PotentialMapHasDimensions(pot, numRows, numCols)
+  requires 0 <= p.pos.row < numRows && 0 <= p.pos.col < numCols
+{
+  (p.pos.row > 0 && pot[p.pos.row - 1][p.pos.col].Real?)
+      || (p.pos.row + 1 < numRows && pot[p.pos.row + 1][p.pos.col].Real?)
+      || (p.pos.col > 0 && pot[p.pos.row][p.pos.col - 1].Real?)
+      || (p.pos.col + 1 < numCols && pot[p.pos.row][p.pos.col + 1].Real?)
+}
+
 predicate ValidQueue(queue: seq<Pose>, pot: PotentialMap, costMap: CostMap)
   requires PotentialMapHasDimensions(pot, costMap.numRows, costMap.numCols)
 {
   forall p: Pose | p in queue ::
     0 <= p.pos.row < costMap.numRows
     && 0 <= p.pos.col < costMap.numCols
-    // && Existe un adyacente en pot que es real
+    && HasSomeAdjacentReal(p, pot, costMap.numRows, costMap.numCols)
 }
 
 method AStar(start: Pose, goal: Pose, costMap: CostMap, numIterations: nat) returns (path: Path)
   requires 0 <= start.pos.row < costMap.numRows && 0 <= start.pos.col < costMap.numCols
   requires 0 <= goal.pos.row < costMap.numRows && 0 <= goal.pos.col < costMap.numCols
   requires open(costMap, goal.pos.row, goal.pos.col)
+  requires ValidCostMap(costMap)
   decreases *
 {
   var pot := BuildInitialPotentialMap(costMap.numRows, costMap.numCols, goal.pos.row, goal.pos.col);
@@ -57,6 +89,7 @@ method AStarIteration(start: Pose, goal: Pose,
                       threshold: real, numIterations: nat) returns (pot': PotentialMap)
   requires ValidPotentialMap(pot, costMap)
   requires ValidQueue(current, pot, costMap) && ValidQueue(next, pot, costMap) && ValidQueue(excess, pot, costMap)
+  requires ValidCostMap(costMap)
   requires 0 <= start.pos.row < costMap.numRows && 0 <= start.pos.col < costMap.numCols
   requires 0 <= goal.pos.row < costMap.numRows && 0 <= goal.pos.col < costMap.numCols
   decreases numIterations, |current|
@@ -76,11 +109,16 @@ method AStarIteration(start: Pose, goal: Pose,
     } else {
       var minV := MinVertical(current[0], pot, costMap.numRows);
       var minH := MinHorizontal(current[0], pot, costMap.numCols);
+      assert minV != Infinity || minH != Infinity;
       var min := MinInfinity(minV, minH);
-      assume min.Real?; // TODO
       var snd := MaxInfinity(minV, minH);
       var potAux := UpdatePotential(pot, current[0], goal, costMap, min, snd);
+      assert ValidQueue(current, potAux, costMap);
+      assert ValidQueue(next, potAux, costMap);
+      assert ValidQueue(excess, potAux, costMap);
       var next', excess' := TraverseNeighbors(current[0], start, costMap, potAux, threshold, next, excess);
+      assert ValidQueue(next', potAux, costMap);
+      assert ValidQueue(excess', potAux, costMap);
       pot' := AStarIteration(start, goal, costMap, potAux, current[1..], next', excess', threshold, numIterations);
     }
   } else {
@@ -100,8 +138,9 @@ method BuildInitialPotentialMap(numRows: nat, numCols: nat, initRow: nat,  initC
 
 
 method InitCurrentQueue(p: Pose, ghost pot: PotentialMap, costMap: CostMap) returns (current: seq<Pose>)
-  requires 0 <= p.pos.row < costMap.numRows && 0 <= p.pos.col < costMap.numCols
   requires PotentialMapHasDimensions(pot, costMap.numRows, costMap.numCols)
+  requires 0 <= p.pos.row < costMap.numRows && 0 <= p.pos.col < costMap.numCols
+  requires pot[p.pos.row][p.pos.col].Real?
   ensures ValidQueue(current, pot, costMap)
 {
   var p1l :=
@@ -118,10 +157,12 @@ method InitCurrentQueue(p: Pose, ghost pot: PotentialMap, costMap: CostMap) retu
 
 method UpdatePotential(pot: PotentialMap, p: Pose, goal: Pose, costMap: CostMap, min: RealInf, snd: RealInf) returns (pot': PotentialMap)
   requires ValidPotentialMap(pot, costMap)
+  requires ValidCostMap(costMap)
   requires 0 <= p.pos.row < costMap.numRows && 0 <= p.pos.col < costMap.numCols
   requires min.Real?
   requires open(costMap, p.pos.row, p.pos.col)
   ensures ValidPotentialMap(pot', costMap)
+  ensures forall i, j | 0 <= i < costMap.numRows && 0 <= j < costMap.numCols && (i != p.pos.row || j != p.pos.col) :: pot'[i][j] == pot[i][j]
   ensures pot'[p.pos.row][p.pos.col].Real?
 {
   var hf := costMap.value(Point(p.pos.row, p.pos.col));
@@ -131,7 +172,6 @@ method UpdatePotential(pot: PotentialMap, p: Pose, goal: Pose, costMap: CostMap,
     pot' := pot[p.pos.row := pot[p.pos.row][p.pos.col := Real(v')]];
   } else {
     assert diff.Real?;
-    assume hf > 0.0;    // TODO
     var d := diff.r / hf;
     var interpol := -0.2301 * d * d + 0.5307 * d + 0.7040;
     var v' := min.r + hf * interpol;
@@ -183,6 +223,7 @@ method TraverseNeighbor(p: Pose, newP: Pose, start: Pose, costMap: CostMap, pot:
   requires ValidPotentialMap(pot, costMap)
   requires 0 <= p.pos.row < costMap.numRows && 0 <= p.pos.col < costMap.numCols
   requires 0 <= newP.pos.row < costMap.numRows && 0 <= newP.pos.col < costMap.numCols
+  requires Adjacent(p, newP, costMap)
   requires pot[p.pos.row][p.pos.col].Real?
   ensures ValidQueue(next', pot, costMap) && ValidQueue(excess', pot, costMap)
 {
@@ -212,25 +253,25 @@ function method Abs(x: int): int {
 method EuclidDistance(p1: Point, p2: Point) returns (d: real) {
   var diffRows := Abs(p1.row - p2.row);
   var diffCols := Abs(p1.col - p2.col);
-  d := (diffRows * diffRows + diffCols * diffCols) as real; // TODO
+  d := (diffRows * diffRows + diffCols * diffCols) as real; // TODO: sqrt?
 }
 
-method MinHorizontal(p: Pose, pot: PotentialMap, numCols: nat) returns (f: RealInf)
+function method MinHorizontal(p: Pose, pot: PotentialMap, numCols: nat): RealInf
   requires exists numRows :: PotentialMapHasDimensions(pot, numRows, numCols) && 0 <= p.pos.row < numRows
   requires 0 <= p.pos.col < numCols
 {
   var left := if p.pos.col > 0 then pot[p.pos.row][p.pos.col - 1] else Infinity;
   var right := if p.pos.col + 1 < numCols then pot[p.pos.row][p.pos.col + 1] else Infinity;
-  f := MinInfinity(left, right);
+  MinInfinity(left, right)
 }
 
-method MinVertical(p: Pose, pot: PotentialMap, numRows: nat) returns (f: RealInf)
+function method MinVertical(p: Pose, pot: PotentialMap, numRows: nat): RealInf
   requires exists numCols :: PotentialMapHasDimensions(pot, numRows, numCols) && 0 <= p.pos.col < numCols
   requires 0 <= p.pos.row < numRows
 {
   var up := if p.pos.row > 0 then pot[p.pos.row - 1][p.pos.col] else Infinity;
   var down := if p.pos.row + 1 < numRows then pot[p.pos.row + 1][p.pos.col] else Infinity;
-  f := MinInfinity(up, down);
+  MinInfinity(up, down)
 }
 
 function method MinInfinity(x1: RealInf, x2: RealInf): RealInf {
